src/Hygge_Theory.thy
@@ -144,6 +144,22 @@ lemma sound_reduction:
        \<lbrakk>\<lbrakk> \<Gamma>\<^sub>2 \<rbrakk>\<rbrakk>\<^sub>s\<^sub>y\<^sub>m\<^sub>r\<^sub>u\<^sub>n \<inter> \<lbrakk>\<lbrakk> \<Psi>\<^sub>2 \<rbrakk>\<rbrakk>\<^sub>T\<^sub>E\<^sub>S\<^sub>L\<^bsup>\<ge> n\<^sub>2\<^esup> \<inter> \<lbrakk>\<lbrakk> \<Phi>\<^sub>2 \<rbrakk>\<rbrakk>\<^sub>T\<^sub>E\<^sub>S\<^sub>L\<^bsup>\<ge> Suc n\<^sub>2\<^esup>
        \<subseteq> \<lbrakk>\<lbrakk> \<Gamma>\<^sub>1 \<rbrakk>\<rbrakk>\<^sub>s\<^sub>y\<^sub>m\<^sub>r\<^sub>u\<^sub>n \<inter> \<lbrakk>\<lbrakk> \<Psi>\<^sub>1 \<rbrakk>\<rbrakk>\<^sub>T\<^sub>E\<^sub>S\<^sub>L\<^bsup>\<ge> n\<^sub>1\<^esup> \<inter> \<lbrakk>\<lbrakk> \<Phi>\<^sub>1 \<rbrakk>\<rbrakk>\<^sub>T\<^sub>E\<^sub>S\<^sub>L\<^bsup>\<ge> Suc n\<^sub>1\<^esup>"
       using HeronConf_interp_stepwise_iff_cases by auto
+    show "\<And>\<Gamma>\<^sub>1' n\<^sub>1' \<Psi>\<^sub>1' \<Phi>\<^sub>1' \<Gamma>\<^sub>2' n\<^sub>2' \<Psi>\<^sub>2' \<Phi>\<^sub>2' \<Gamma> n master slave \<Psi> \<Phi> K\<^sub>1.
+       \<Gamma>\<^sub>1, n\<^sub>1 \<turnstile> \<Psi>\<^sub>1 \<triangleright> \<Phi>\<^sub>1 = \<Gamma>\<^sub>1', n\<^sub>1' \<turnstile> \<Psi>\<^sub>1' \<triangleright> \<Phi>\<^sub>1' \<Longrightarrow>
+       \<Gamma>\<^sub>2, n\<^sub>2 \<turnstile> \<Psi>\<^sub>2 \<triangleright> \<Phi>\<^sub>2 = \<Gamma>\<^sub>2', n\<^sub>2' \<turnstile> \<Psi>\<^sub>2' \<triangleright> \<Phi>\<^sub>2' \<Longrightarrow>
+       \<Gamma>\<^sub>1', n\<^sub>1' \<turnstile> \<Psi>\<^sub>1' \<triangleright> \<Phi>\<^sub>1' = \<Gamma>, n \<turnstile> (master anytime implies slave) # \<Psi> \<triangleright> \<Phi> \<Longrightarrow>
+       \<Gamma>\<^sub>2', n\<^sub>2' \<turnstile> \<Psi>\<^sub>2' \<triangleright> \<Phi>\<^sub>2' = (master \<not>\<Up> n) # \<Gamma>, n \<turnstile> \<Psi> \<triangleright> (master anytime implies slave) # \<Phi> \<Longrightarrow>
+       \<lbrakk>\<lbrakk> \<Gamma>\<^sub>2 \<rbrakk>\<rbrakk>\<^sub>s\<^sub>y\<^sub>m\<^sub>r\<^sub>u\<^sub>n \<inter> \<lbrakk>\<lbrakk> \<Psi>\<^sub>2 \<rbrakk>\<rbrakk>\<^sub>T\<^sub>E\<^sub>S\<^sub>L\<^bsup>\<ge> n\<^sub>2\<^esup> \<inter> \<lbrakk>\<lbrakk> \<Phi>\<^sub>2 \<rbrakk>\<rbrakk>\<^sub>T\<^sub>E\<^sub>S\<^sub>L\<^bsup>\<ge> Suc n\<^sub>2\<^esup>
+       \<subseteq> \<lbrakk>\<lbrakk> \<Gamma>\<^sub>1 \<rbrakk>\<rbrakk>\<^sub>s\<^sub>y\<^sub>m\<^sub>r\<^sub>u\<^sub>n \<inter> \<lbrakk>\<lbrakk> \<Psi>\<^sub>1 \<rbrakk>\<rbrakk>\<^sub>T\<^sub>E\<^sub>S\<^sub>L\<^bsup>\<ge> n\<^sub>1\<^esup> \<inter> \<lbrakk>\<lbrakk> \<Phi>\<^sub>1 \<rbrakk>\<rbrakk>\<^sub>T\<^sub>E\<^sub>S\<^sub>L\<^bsup>\<ge> Suc n\<^sub>1\<^esup>"
+      sorry
+    show "\<And>\<Gamma>\<^sub>1' n\<^sub>1' \<Psi>\<^sub>1' \<Phi>\<^sub>1' \<Gamma>\<^sub>2' n\<^sub>2' \<Psi>\<^sub>2' \<Phi>\<^sub>2' \<Gamma> n master slave \<Psi> \<Phi>.
+       \<Gamma>\<^sub>1, n\<^sub>1 \<turnstile> \<Psi>\<^sub>1 \<triangleright> \<Phi>\<^sub>1 = \<Gamma>\<^sub>1', n\<^sub>1' \<turnstile> \<Psi>\<^sub>1' \<triangleright> \<Phi>\<^sub>1' \<Longrightarrow>
+       \<Gamma>\<^sub>2, n\<^sub>2 \<turnstile> \<Psi>\<^sub>2 \<triangleright> \<Phi>\<^sub>2 = \<Gamma>\<^sub>2', n\<^sub>2' \<turnstile> \<Psi>\<^sub>2' \<triangleright> \<Phi>\<^sub>2' \<Longrightarrow>
+       \<Gamma>\<^sub>1', n\<^sub>1' \<turnstile> \<Psi>\<^sub>1' \<triangleright> \<Phi>\<^sub>1' = \<Gamma>, n \<turnstile> (master anytime implies slave) # \<Psi> \<triangleright> \<Phi> \<Longrightarrow>
+       \<Gamma>\<^sub>2', n\<^sub>2' \<turnstile> \<Psi>\<^sub>2' \<triangleright> \<Phi>\<^sub>2' = (master \<Up> n) # \<Gamma>, n \<turnstile> (slave sporadic anytime) # \<Psi> \<triangleright> (master anytime implies slave) # \<Phi> \<Longrightarrow>
+       \<lbrakk>\<lbrakk> \<Gamma>\<^sub>2 \<rbrakk>\<rbrakk>\<^sub>s\<^sub>y\<^sub>m\<^sub>r\<^sub>u\<^sub>n \<inter> \<lbrakk>\<lbrakk> \<Psi>\<^sub>2 \<rbrakk>\<rbrakk>\<^sub>T\<^sub>E\<^sub>S\<^sub>L\<^bsup>\<ge> n\<^sub>2\<^esup> \<inter> \<lbrakk>\<lbrakk> \<Phi>\<^sub>2 \<rbrakk>\<rbrakk>\<^sub>T\<^sub>E\<^sub>S\<^sub>L\<^bsup>\<ge> Suc n\<^sub>2\<^esup>
+       \<subseteq> \<lbrakk>\<lbrakk> \<Gamma>\<^sub>1 \<rbrakk>\<rbrakk>\<^sub>s\<^sub>y\<^sub>m\<^sub>r\<^sub>u\<^sub>n \<inter> \<lbrakk>\<lbrakk> \<Psi>\<^sub>1 \<rbrakk>\<rbrakk>\<^sub>T\<^sub>E\<^sub>S\<^sub>L\<^bsup>\<ge> n\<^sub>1\<^esup> \<inter> \<lbrakk>\<lbrakk> \<Phi>\<^sub>1 \<rbrakk>\<rbrakk>\<^sub>T\<^sub>E\<^sub>S\<^sub>L\<^bsup>\<ge> Suc n\<^sub>1\<^esup>"
+      sorry
     show "\<And>\<Gamma>\<^sub>1' n\<^sub>1' \<Psi>\<^sub>1' \<Phi>\<^sub>1' \<Gamma>\<^sub>2' n\<^sub>2' \<Psi>\<^sub>2' \<Phi>\<^sub>2' \<Gamma> n K\<^sub>1 \<delta>\<tau> K\<^sub>2 K\<^sub>3 \<Psi> \<Phi>.
        (\<Gamma>\<^sub>1, n\<^sub>1 \<turnstile> \<Psi>\<^sub>1 \<triangleright> \<Phi>\<^sub>1) = (\<Gamma>\<^sub>1', n\<^sub>1' \<turnstile> \<Psi>\<^sub>1' \<triangleright> \<Phi>\<^sub>1') \<Longrightarrow>
        (\<Gamma>\<^sub>2, n\<^sub>2 \<turnstile> \<Psi>\<^sub>2 \<triangleright> \<Phi>\<^sub>2) = (\<Gamma>\<^sub>2', n\<^sub>2' \<turnstile> \<Psi>\<^sub>2' \<triangleright> \<Phi>\<^sub>2') \<Longrightarrow>
@@ -255,6 +271,10 @@ lemma complete_direct_successors:
         case (Iff K1 K2)
         then show ?case
           by (smt Cnext_solve_iff HeronConf_interp_stepwise_iff_cases UN_iff UnE insert_subset subsetI)
+      next
+        case (ImpliesAnytime K1 K2)
+        then show ?case
+          by (smt Cnext_solve_implies_anytime HeronConf_interp_stepwise_implies_anytime_cases UN_iff UnE insert_subset subsetI)
       next
         case (TimeDelayedBy Kmast \<tau> Kmeas Kslave)
         then show ?case
@@ -435,6 +455,10 @@ lemma instant_index_increase:
       then show ?case
         by (metis (no_types, lifting) HeronConf_interp_stepwise_iff_cases Un_iff elims_part iff_e1 iff_e2 relpowp_Suc_I2)
     next
+      case (ImpliesAnytime master slave)
+      then show ?case
+        sorry
+    next
       case (TimeDelayedBy K\<^sub>1 \<delta>\<tau> K\<^sub>2 K\<^sub>3)
       have branches: "\<lbrakk> \<Gamma>, n \<turnstile> (K\<^sub>1 time-delayed by \<delta>\<tau> on K\<^sub>2 implies K\<^sub>3) # \<Psi> \<triangleright> \<Phi> \<rbrakk>\<^sub>c\<^sub>o\<^sub>n\<^sub>f\<^sub>i\<^sub>g
           = \<lbrakk> K\<^sub>1 \<not>\<Up> n # \<Gamma>, n \<turnstile> \<Psi> \<triangleright> (K\<^sub>1 time-delayed by \<delta>\<tau> on K\<^sub>2 implies K\<^sub>3) # \<Phi> \<rbrakk>\<^sub>c\<^sub>o\<^sub>n\<^sub>f\<^sub>i\<^sub>g
@@ -534,8 +558,9 @@ section \<open>Local termination\<close>
 primrec measure_interpretation :: "TESL_formula \<Rightarrow> nat" ("\<mu>") where
     "\<mu> [] = (0::nat)"
   | "\<mu> (\<phi> # \<Phi>) = (case \<phi> of
-                        _ sporadic _ on _ \<Rightarrow> 1 + \<mu> \<Phi>
-                      | _                 \<Rightarrow> 2 + \<mu> \<Phi>)"
+                        _ sporadic _ on _  \<Rightarrow> 1 + \<mu> \<Phi>
+                      | _ sporadic anytime \<Rightarrow> 1 + \<mu> \<Phi>
+                      | _                  \<Rightarrow> 2 + \<mu> \<Phi>)"
 
 fun measure_interpretation_config :: "config \<Rightarrow> nat" ("\<mu>\<^sub>c\<^sub>o\<^sub>n\<^sub>f\<^sub>i\<^sub>g") where
     "\<mu>\<^sub>c\<^sub>o\<^sub>n\<^sub>f\<^sub>i\<^sub>g (\<Gamma>, n \<turnstile> \<Psi> \<triangleright> \<Phi>) = \<mu> \<Psi>"
